simulations/hmodsim/HPSimFacts.v
@@ -6,6 +6,7 @@ Require Import PCM IModL.
 Require Import Any.
 Require Import STB ModSim.
 Require Import Events HMod HMod2Mod.
+Require Import ModSimTactics.
 
 Require Import Relation_Definitions.
 
@@ -98,89 +99,103 @@ Section HPSIM_ADD_DUMMY.
       esplits; grind; eauto; try by econs; eauto 10.
     - assert (CASE:= case_itrH _ i); des; subst; itree_clarify DUMMY.
       rewrite <-x; destruct with_dummy; grind; econs; eauto with imodL.
-      i. econs. ii. esplits; eauto. econs; eauto with imodL.
+      econs. ii. esplits; eauto. econs; eauto with imodL.
+      i. econs. econs. esplits; eauto. econs; eauto with imodL.
     - assert (CASE:= case_itrH _ i); des; subst; itree_clarify DUMMY.
       + rewrite -x -(bind_ret_l_eta _ k_src) -bind_vis.
         destruct with_dummy; grind; eauto using @_hpsim'.
-        eapply hpsim_guarantee_src; try econs; eauto with imodL.
-        ii; esplits; eauto. econs; eauto.
+        eapply hpsim_guarantee_src; try econs; eauto with imodL. ii; esplits; eauto.
+        eapply hpsim_tau_src; eauto. econs; ii; esplits; eauto.
+        econs; eauto.
       + replace c with (Call fn varg). econs; eauto.
     - assert (CASE:= case_itrH _ i); des; subst; itree_clarify DUMMY.
       + rewrite -x -(bind_ret_l_eta _ k_src) -bind_vis.
         destruct with_dummy; grind; eauto using @_hpsim'.
-        eapply hpsim_guarantee_src; try econs; eauto with imodL.
-        ii. esplits; eauto. econs; eauto.
+        eapply hpsim_guarantee_src; try econs; eauto with imodL. ii. esplits; eauto.
+        eapply hpsim_tau_src; eauto. econs; ii; esplits; eauto.
+        econs; eauto.
       + replace e with (@IO I R0 fn varg). econs; eauto.
     - assert (CASE:= case_itrH _ i); des; subst; itree_clarify DUMMY.
       + rewrite -x -(bind_ret_l_eta _ k_src) -bind_vis.
         destruct with_dummy; grind; eauto using @_hpsim'.
-        eapply hpsim_guarantee_src; try econs; eauto with imodL.
-        ii. esplits; eauto. econs; eauto.
+        eapply hpsim_guarantee_src; try econs; eauto with imodL. ii. esplits; eauto.
+        eapply hpsim_tau_src; eauto. econs; ii; esplits; eauto.
+        econs; eauto.
       + replace c with (Call fn varg). econs; eauto. eapply K; eauto.
-        eexists with_dummy, _, (x<-f varg;; trigger (Guarantee True);;; ktrH' x), k.
+        eexists with_dummy, _, (x<-f varg;; trigger (Guarantee True);;; tau;; ktrH' x), k.
         esplits; grind.
     - assert (CASE:= case_itrH _ i); des; subst; itree_clarify DUMMY.
       + rewrite -x. destruct with_dummy; grind; eauto using @_hpsim'.
-        eapply hpsim_guarantee_src; eauto with imodL.
-        ii. econs. ii. esplits; eauto. econs; eauto.
+        eapply hpsim_guarantee_src; eauto with imodL. ii. econs. ii. esplits; eauto.
+        eapply hpsim_tau_src; eauto. econs; ii; esplits; eauto.
+        econs; eauto.
       + econs; eauto.
     - assert (CASE:= case_itrH _ i); des; subst; itree_clarify DUMMY.
       + rewrite -x -(bind_ret_l_eta _ k_src) -bind_vis.
         destruct with_dummy; grind; eauto using @_hpsim'.
-        eapply hpsim_guarantee_src; eauto with imodL.
-        ii. econs. ii. esplits; eauto. econs; eauto.
+        eapply hpsim_guarantee_src; eauto with imodL. ii. econs. ii. esplits; eauto.
+        eapply hpsim_tau_src; eauto. econs; ii; esplits; eauto.
+        econs; eauto.
       + replace e with (Take R0); econs; eauto.
     - assert (CASE:= case_itrH _ i); des; subst; itree_clarify DUMMY.
       + rewrite -x -(bind_ret_l_eta _ k_src) -bind_vis.
         destruct with_dummy; grind; eauto using @_hpsim'.
-        eapply hpsim_guarantee_src; eauto with imodL.
-        ii. econs. ii. esplits; eauto. econs; eauto.
+        eapply hpsim_guarantee_src; eauto with imodL. ii. econs. ii. esplits; eauto.
+        eapply hpsim_tau_src; eauto. econs; ii; esplits; eauto.
+        econs; eauto.
       + replace e with (Choose R0); eauto. econs; eauto.
     - assert (CASE:= case_itrH _ i); des; subst; itree_clarify DUMMY.
       + rewrite -x -(bind_ret_l_eta _ k_src) -bind_vis.
         destruct with_dummy; grind; eauto using @_hpsim'.
-        eapply hpsim_guarantee_src; eauto with imodL.
-        ii. econs. ii. esplits; eauto. econs; eauto.
+        eapply hpsim_guarantee_src; eauto with imodL. ii. econs. ii. esplits; eauto.
+        eapply hpsim_tau_src; eauto. econs; ii; esplits; eauto.
+        econs; eauto.
       + depdes s; depdes x.
         * econs; eauto.
         * exfalso. apply any_neq_unit; eauto.
     - assert (CASE:= case_itrH _ i); des; subst; itree_clarify DUMMY.
       + rewrite -x -(bind_ret_l_eta _ k_src) -bind_vis.
-        destruct with_dummy; grind; eauto using @_hpsim'. 
-        eapply hpsim_guarantee_src; eauto with imodL.
-        ii. econs. ii. esplits; eauto. econs; eauto.
+        destruct with_dummy; grind; eauto using @_hpsim'.
+        eapply hpsim_guarantee_src; eauto with imodL. ii. econs. ii. esplits; eauto.
+        eapply hpsim_tau_src; eauto. econs; ii; esplits; eauto.
+        econs; eauto.
       + depdes s; depdes x.
         * exfalso. apply any_neq_unit; eauto.
         * econs; eauto.
     - assert (CASE:= case_itrH _ i); des; subst; itree_clarify DUMMY.
       + rewrite -x -(bind_ret_l_eta _ k_src) -bind_vis.
         destruct with_dummy; grind; eauto using @_hpsim'.
-        eapply hpsim_guarantee_src; eauto with imodL.
-        ii. econs. ii. esplits; eauto. econs; eauto.
+        eapply hpsim_guarantee_src; eauto with imodL. ii. econs. ii. esplits; eauto.
+        eapply hpsim_tau_src; eauto. econs; ii; esplits; eauto.
+        econs; eauto.
       + econs; eauto.
     - assert (CASE:= case_itrH _ i); des; subst; itree_clarify DUMMY.
       + rewrite -x -(bind_ret_l_eta _ k_src) -bind_vis.
         destruct with_dummy; grind; eauto using @_hpsim'.
-        eapply hpsim_guarantee_src; eauto with imodL.
-        ii. econs. ii. esplits; eauto. econs; eauto.
+        eapply hpsim_guarantee_src; eauto with imodL. ii. econs. ii. esplits; eauto.
+        eapply hpsim_tau_src; eauto. econs; ii; esplits; eauto.
+        econs; eauto.
       + econs; eauto.
     - assert (CASE:= case_itrH _ i); des; subst; itree_clarify DUMMY.
       + rewrite -x -(bind_ret_l_eta _ k_src) -bind_vis.
         destruct with_dummy; grind; eauto using @_hpsim'.
-        eapply hpsim_guarantee_src; try econs; eauto with imodL.
-        ii. esplits; eauto. econs; eauto.
+        eapply hpsim_guarantee_src; try econs; eauto with imodL. ii. esplits; eauto.
+        eapply hpsim_tau_src; eauto. econs; ii; esplits; eauto.
+        econs; eauto.
       + replace s with (Spawn fn arg). econs; eauto.
     - assert (CASE:= case_itrH _ i); des; subst; itree_clarify DUMMY.
       + rewrite -x -(bind_ret_l_eta _ k_src) -bind_vis.
         destruct with_dummy; grind; eauto using @_hpsim'.
-        eapply hpsim_guarantee_src; try econs; eauto with imodL.
-        ii; esplits; eauto. econs; eauto.
+        eapply hpsim_guarantee_src; try econs; eauto with imodL. ii; esplits; eauto.
+        eapply hpsim_tau_src; eauto. econs; ii; esplits; eauto.
+        econs; eauto.
       + replace s with (Yield tid). econs; eauto.
     - assert (CASE:= case_itrH _ i); des; subst; itree_clarify DUMMY.
       + rewrite -x -(bind_ret_l_eta _ k_src) -bind_vis.
         destruct with_dummy; grind; eauto using @_hpsim'.
-        eapply hpsim_guarantee_src; try econs; eauto with imodL.
-        ii; esplits; eauto. econs; eauto.
+        eapply hpsim_guarantee_src; try econs; eauto with imodL. ii; esplits; eauto.
+        eapply hpsim_tau_src; eauto. econs; ii; esplits; eauto.
+        econs; eauto.
       + replace s with Tid. econs; eauto.
     - econs; eauto. econs; eauto.
   Qed.
@@ -224,89 +239,103 @@ Section HPSIM_ADD_DUMMY.
       esplits; grind; eauto; try by econs; eauto 10.
     - assert (CASE:= case_itrH _ i); des; subst; itree_clarify DUMMY.
       rewrite <-x; destruct with_dummy; grind; econs; eauto; imodIntroL.
+      econs. ii. esplits; eauto. econs; eauto with imodL.
       i. econs. ii. esplits; eauto. econs; eauto; imodIntroL.
     - assert (CASE:= case_itrH _ i); des; subst; itree_clarify DUMMY.
       + rewrite -x -(bind_ret_l_eta _ k_tgt) -bind_vis.
         destruct with_dummy; grind; eauto using @_hpsim'.
-        eapply hpsim_guarantee_tgt; try econs; eauto; imodIntroL.
-        ii; esplits; eauto. econs; eauto.
+        eapply hpsim_guarantee_tgt; try econs; eauto; imodIntroL. ii; esplits; eauto.
+        eapply hpsim_tau_tgt; eauto. econs; ii; esplits; eauto.
+        econs; eauto.
       + replace c with (Call fn varg). econs; eauto.
     - assert (CASE:= case_itrH _ i); des; subst; itree_clarify DUMMY.
       + rewrite -x -(bind_ret_l_eta _ k_tgt) -bind_vis.
         destruct with_dummy; grind; eauto using @_hpsim'.
-        eapply hpsim_guarantee_tgt; try econs; eauto; imodIntroL.
-        ii. esplits; eauto. econs; eauto.
+        eapply hpsim_guarantee_tgt; try econs; eauto; imodIntroL. ii. esplits; eauto.
+        eapply hpsim_tau_tgt; eauto. econs; ii; esplits; eauto.
+        econs; eauto.
       + replace e with (@IO I R0 fn varg). econs; eauto.
     - assert (CASE:= case_itrH _ i); des; subst; itree_clarify DUMMY.
       + rewrite -x -(bind_ret_l_eta _ k_tgt) -bind_vis.
         destruct with_dummy; grind; eauto using @_hpsim'.
-        eapply hpsim_guarantee_tgt; try econs; eauto; imodIntroL.
-        ii. esplits; eauto. econs; eauto.
+        eapply hpsim_guarantee_tgt; try econs; eauto; imodIntroL. ii. esplits; eauto.
+        eapply hpsim_tau_tgt; eauto. econs; ii; esplits; eauto.
+        econs; eauto.
       + replace c with (Call fn varg). econs; eauto. eapply K; eauto.
-        eexists with_dummy, _, (x<-f varg;; trigger (Guarantee True);;; ktrH' x), k.
+        eexists with_dummy, _, (x<-f varg;; trigger (Guarantee True);;; tau;; ktrH' x), k.
         esplits; grind.
     - assert (CASE:= case_itrH _ i); des; subst; itree_clarify DUMMY.
       + rewrite -x. destruct with_dummy; grind; eauto using @_hpsim'.
-        eapply hpsim_guarantee_tgt; eauto; imodIntroL.
-        ii. econs. ii. esplits; eauto. econs; eauto.
+        eapply hpsim_guarantee_tgt; eauto; imodIntroL. ii. econs. ii. esplits; eauto.
+        eapply hpsim_tau_tgt; eauto. econs; ii; esplits; eauto.
+        econs; eauto.
       + econs; eauto.
     - assert (CASE:= case_itrH _ i); des; subst; itree_clarify DUMMY.
       + rewrite -x -(bind_ret_l_eta _ k_tgt) -bind_vis.
         destruct with_dummy; grind; eauto using @_hpsim'.
-        eapply hpsim_guarantee_tgt; eauto; imodIntroL.
-        ii. econs. ii. esplits; eauto. econs; eauto.
+        eapply hpsim_guarantee_tgt; eauto; imodIntroL. ii. econs. ii. esplits; eauto.
+        eapply hpsim_tau_tgt; eauto. econs; ii; esplits; eauto.
+        econs; eauto.
       + replace e with (Choose R0); econs; eauto.
     - assert (CASE:= case_itrH _ i); des; subst; itree_clarify DUMMY.
       + rewrite -x -(bind_ret_l_eta _ k_tgt) -bind_vis.
         destruct with_dummy; grind; eauto using @_hpsim'.
-        eapply hpsim_guarantee_tgt; eauto; imodIntroL.
-        ii. econs. ii. esplits; eauto. econs; eauto.
+        eapply hpsim_guarantee_tgt; eauto; imodIntroL. ii. econs. ii. esplits; eauto.
+        eapply hpsim_tau_tgt; eauto. econs; ii; esplits; eauto.
+        econs; eauto.
       + replace e with (Take R0); eauto. econs; eauto.
     - assert (CASE:= case_itrH _ i); des; subst; itree_clarify DUMMY.
       + rewrite -x -(bind_ret_l_eta _ k_tgt) -bind_vis.
         destruct with_dummy; grind; eauto using @_hpsim'.
-        eapply hpsim_guarantee_tgt; eauto; imodIntroL.
-        ii. econs. ii. esplits; eauto. econs; eauto.
+        eapply hpsim_guarantee_tgt; eauto; imodIntroL. ii. econs. ii. esplits; eauto.
+        eapply hpsim_tau_tgt; eauto. econs; ii; esplits; eauto.
+        econs; eauto.
       + depdes s; depdes x.
         * econs; eauto.
         * exfalso. apply any_neq_unit; eauto.
     - assert (CASE:= case_itrH _ i); des; subst; itree_clarify DUMMY.
       + rewrite -x -(bind_ret_l_eta _ k_tgt) -bind_vis.
         destruct with_dummy; grind; eauto using @_hpsim'.
-        eapply hpsim_guarantee_tgt; eauto; imodIntroL.
-        ii. econs. ii. esplits; eauto. econs; eauto.
+        eapply hpsim_guarantee_tgt; eauto; imodIntroL. ii. econs. ii. esplits; eauto.
+        eapply hpsim_tau_tgt; eauto. econs; ii; esplits; eauto.
+        econs; eauto.
       + depdes s; depdes x.
         * exfalso. apply any_neq_unit; eauto.
         * econs; eauto.
     - assert (CASE:= case_itrH _ i); des; subst; itree_clarify DUMMY.
       + rewrite -x -(bind_ret_l_eta _ k_tgt) -bind_vis.
-        destruct with_dummy; grind; eauto using @_hpsim'. 
-        eapply hpsim_guarantee_tgt; eauto; imodIntroL.
-        ii. econs. ii. esplits; eauto. econs; eauto.
+        destruct with_dummy; grind; eauto using @_hpsim'.
+        eapply hpsim_guarantee_tgt; eauto; imodIntroL. ii. econs. ii. esplits; eauto.
+        eapply hpsim_tau_tgt; eauto. econs; ii; esplits; eauto.
+        econs; eauto.
       + econs; eauto.
     - assert (CASE:= case_itrH _ i); des; subst; itree_clarify DUMMY.
       + rewrite -x -(bind_ret_l_eta _ k_tgt) -bind_vis.
         destruct with_dummy; grind; eauto using @_hpsim'.
-        eapply hpsim_guarantee_tgt; eauto; imodIntroL.
-        ii. econs. ii. esplits; eauto. econs; eauto.
+        eapply hpsim_guarantee_tgt; eauto; imodIntroL. ii. econs. ii. esplits; eauto.
+        eapply hpsim_tau_tgt; eauto. econs; ii; esplits; eauto.
+        econs; eauto.
       + econs; eauto.
     - assert (CASE:= case_itrH _ i); des; subst; itree_clarify DUMMY.
       + rewrite -x -(bind_ret_l_eta _ k_tgt) -bind_vis.
         destruct with_dummy; grind; eauto using @_hpsim'.
-        eapply hpsim_guarantee_tgt; try econs; eauto; imodIntroL.
-        ii. esplits; eauto. econs; eauto.
+        eapply hpsim_guarantee_tgt; try econs; eauto; imodIntroL. ii. esplits; eauto.
+        eapply hpsim_tau_tgt; eauto. econs; ii; esplits; eauto.
+        econs; eauto.
       + replace s with (Spawn fn arg). econs; eauto.
     - assert (CASE:= case_itrH _ i); des; subst; itree_clarify DUMMY.
       + rewrite -x -(bind_ret_l_eta _ k_tgt) -bind_vis.
         destruct with_dummy; grind; eauto using @_hpsim'.
-        eapply hpsim_guarantee_tgt; try econs; eauto; imodIntroL.
-        ii. esplits; eauto. econs; eauto.
+        eapply hpsim_guarantee_tgt; try econs; eauto; imodIntroL. ii. esplits; eauto.
+        eapply hpsim_tau_tgt; eauto. econs; ii; esplits; eauto.
+        econs; eauto.
       + replace s with (Yield tid). econs; eauto.
     - assert (CASE:= case_itrH _ i); des; subst; itree_clarify DUMMY.
       + rewrite -x -(bind_ret_l_eta _ k_tgt) -bind_vis.
         destruct with_dummy; grind; eauto using @_hpsim'.
-        eapply hpsim_guarantee_tgt; try econs; eauto; imodIntroL.
-        ii. esplits; eauto. econs; eauto.
+        eapply hpsim_guarantee_tgt; try econs; eauto; imodIntroL. ii. esplits; eauto.
+        eapply hpsim_tau_tgt; eauto. econs; ii; esplits; eauto.
+        econs; eauto.
       + replace s with Tid. econs; eauto.
     - subst. econs; eauto. econs; eauto.
   Qed.
@@ -338,9 +367,6 @@ Section HPSIM_ADD_DUMMY.
   Proof. ginit. i. eapply hpsim_le_gpaco. eauto. Qed.
 
 End HPSIM_ADD_DUMMY.
-
-
-
 
 Section INTERP_RECONF.
 
@@ -479,7 +505,10 @@ Section INTERP_RECONF.
     sim_strict my_tid _ (fun _ => hp_reconf_rel R hp_reconf_equiv cr) nths
       (str, interp_hp itrH fr)
       (str', interp_hp itrH fr').
-    Proof.
+  Proof.
+    (* A workaround for a bug in Qed *)
+    assert (BUGFIX := @handle_Guarantee_reconf). move BUGFIX at top.
+    
     revert_until Ist. ginit. gcofix CIH; i.
     assert (CASE := case_itrH _ itrH). des; subst.
     - rewrite !interp_hp_ret.
@@ -507,8 +536,18 @@ Section INTERP_RECONF.
         eapply handle_Guarantee_reconf. eauto. }
       i. grind; gstep; econs; i.
       gfinal. left. eapply CIH. destruct v0, v0'. rr in REL. des; subst. ss.
-    - admit.
-      
+    - destruct s.
+      + rewrite-> !interp_hp_bind, !interp_hp_spawn.
+        repeat (grind; gstep; econs; i). gbase. eauto.
+      + rewrite-> !interp_hp_bind, !interp_hp_yield. grind.
+        guclo sim_strict_bindC_spec. econs.
+        { gfinal. right. eapply paco5_mon_bot; eauto.
+          eapply handle_Guarantee_reconf_true. eauto. }
+        i. destruct v0, v0'. repeat (rr in REL; des; subst).
+        repeat (grind; gstep; econs; i).
+        gfinal. left. eapply CIH. left. s. eauto.
+      + rewrite-> !interp_hp_bind, !interp_hp_tid.
+        repeat (grind; gstep; econs; i). gbase. eauto.
     - rewrite-> !interp_hp_bind, !interp_hp_call. grind.
       guclo sim_strict_bindC_spec. econs.
       { gfinal. right. eapply paco5_mon_bot; eauto.
@@ -517,24 +556,24 @@ Section INTERP_RECONF.
       repeat (grind; gstep; econs; i).
       gfinal. left. eapply CIH. left. s. eauto.
     - rewrite-> !interp_hp_bind, !interp_hp_pg.
-      destruct s. 
-      + unfold handle_pgE_tgt, mput_kv.
+      destruct s.
+      + unfold handle_pgE, mput_kv.
         repeat (grind; gstep; econs; i).
         grind; apply hp_reconf_equiv_strong in RELr; repeat (rr in RELr; des; subst); cycle 1.
         { rewrite !Any.pair_split. repeat (grind; gstep; econs).
           gfinal. left. eapply CIH. right. esplits; eauto. }
         destruct (Any.split str) as [[]|] eqn: STR; cycle 1.
-        { s. unfold triggerUB. grind. gstep. econs. i. ss. }        
+        { s. unfold triggerUB. grind. gstep. econs. i. ss. }
         apply Any.split_pair in STR. des; subst.
         repeat (grind; gstep; econs).
         gfinal. left. eapply CIH. econs. econs; eauto.
-      + unfold handle_pgE_tgt, mget_kv.
+      + unfold handle_pgE, mget_kv.
         repeat (grind; gstep; econs; i).
         grind; apply hp_reconf_equiv_strong in RELr; repeat (rr in RELr; des; subst); cycle 1.
         { rewrite !Any.pair_split. repeat (grind; gstep; econs).
           gfinal. left. eapply CIH. right. esplits; eauto. }
         destruct (Any.split str) as [[]|] eqn: STR; cycle 1.
-        { s. unfold triggerUB. grind. gstep. econs. i. ss. }        
+        { s. unfold triggerUB. grind. gstep. econs. i. ss. }
         apply Any.split_pair in STR. des; subst.
         repeat (grind; gstep; econs).
         gfinal. left. eapply CIH. econs. econs; eauto.
@@ -545,7 +584,7 @@ Section INTERP_RECONF.
       + grind; gstep; econs; i. eexists.
         repeat (grind; gstep; econs; i). eauto 10 with paco.
       + repeat (grind; gstep; econs; i). eauto 10 with paco.
-    Admitted.
+  Qed.
 
   Lemma hp_fun_tail_reconf
     nths str str' (fr fr' cr: Σ) x
@@ -582,8 +621,8 @@ Section INTERP_RECONF.
     nths itrH ktrH st (fr mr: Σ)
     :
     sim_strict my_tid Any.t (fun _ => eq) nths
-      (Any.pair st (fr ⋅ mr)↑, x <- interp_hp_body itrH ε;; '(rr,rv) <- (tau;; Ret (ε,x));; interp_hp_body (ktrH rv) rr)
-      (Any.pair st mr↑, interp_hp_body (x <- itrH;; trigger (Guarantee True) ;;; ktrH x) fr).
+      (Any.pair st (fr ⋅ mr)↑, x <- interp_hp_body itrH ε;; tau;; '(rr,rv) <- (tau;; Ret (ε,x));; interp_hp_body (ktrH rv) rr)
+      (Any.pair st mr↑, interp_hp_body (x <- itrH;; trigger (Guarantee True);;; tau;; ktrH x) fr).
   Proof.
     ginit. guclo sim_strict_transC_spec. econs; cycle 1.
     { gfinal. right. eapply interp_hp_body_reconf with (fr := (ε:Σ)) (cr:=(ε:Σ)).
@@ -606,7 +645,7 @@ Section INTERP_RECONF.
     grind; gstep; econs; i. eexists. { r_solve. eauto. }
     grind; gstep; econs; i. eexists. { eauto. }
     repeat (grind; gstep; econs; i).
-    grind. rewrite !Any.pair_split.
+    grind. rewrite/__ !Any.pair_split interp_hp_tau.
     repeat (grind; gstep; econs; i).
     gfinal. right. eapply interp_hp_body_reconf with (cr:=(ε:Σ)).
     right. esplits; eauto. r_solve. eauto.
@@ -617,8 +656,8 @@ Section INTERP_RECONF.
     (RELr: Own (fr ⋅ mr) ⊢ #=> Own (fr' ⋅ mr'))
     :
     sim_strict my_tid Any.t (fun _ => eq) nths
-      (Any.pair st mr↑, interp_hp_body (x <- itrH;; trigger (Guarantee True) ;;; ktrH x) fr)
-      (Any.pair st mr'↑, x <- interp_hp_body itrH ε;; '(rr,rv) <- (tau;; Ret (fr',x));; interp_hp_body (ktrH rv) rr).
+      (Any.pair st mr↑, interp_hp_body (x <- itrH;; trigger (Guarantee True) ;;; tau;; ktrH x) fr)
+      (Any.pair st mr'↑, x <- interp_hp_body itrH ε;; tau;; '(rr,rv) <- (tau;; Ret (fr',x));; interp_hp_body (ktrH rv) rr).
   Proof.
     ginit. unfold interp_hp_body. rewrite-> !interp_hp_bind. grind.
     guclo sim_strict_bindC_spec. econs.
@@ -630,7 +669,7 @@ Section INTERP_RECONF.
     { gfinal. right. eapply handle_Guarantee_reconf_true.
       destruct v0. ss. des; subst; eauto.
       right. esplits; eauto. }
-    i. grind; gstep; econs; i.
+    i. grind; gstep; econs; i. rewrite interp_hp_tau. grind. gstep. econs; i.
     destruct v0. rr in REL; des; subst. simpl. destruct v1, v0'.
     guclo sim_strict_bindC_spec. econs.
     { gfinal. right.  eapply interp_hp_reconf with (cr:=c2).
@@ -640,7 +679,7 @@ Section INTERP_RECONF.
     { gfinal. right. eapply handle_Guarantee_reconf_true.
       r in REL1. des; subst. eauto. }
     i. gstep; econs. rr in REL1. des; subst.
-    destruct v0, v0'. s in REL2; des; subst. eauto. 
+    destruct v0, v0'. s in REL2; des; subst. eauto.
   Qed.
 
 End INTERP_RECONF.
@@ -679,18 +718,83 @@ Section HPSIM_ADEQUACY.
     iModIntro. iSplitR "MRT"; eauto. iSplitR "FRT"; eauto. iSplitR "FMR"; eauto.
   Qed.
 
+  Definition ctx_sem (ctx: list Σ) : Σ :=
+    foldr URA.add ε ctx.
+
+  Definition ctx_set (ctx: list Σ) (r: Σ) : list Σ :=
+    <[my_tid := r]> ctx.
+  
+  Definition ctx_add (ctx: list Σ) (r: Σ) : list Σ :=
+    ctx_set ctx ((or_else (ctx !! my_tid) ε) ⋅ r).
+
+  Lemma ctx_set_sem ctx r r'
+    (IN: my_tid < List.length ctx):
+    ctx_sem (ctx_set ctx (r ⋅ r')) = ctx_sem (ctx_set ctx r) ⋅ r'.
+  Proof.
+    unfold ctx_set. revert my_tid r r' IN.
+    induction ctx; i; ss; try nia.
+    destruct my_tid; s; r_solve.
+    eapply IHctx; try nia.
+  Qed.
+  
+  Lemma ctx_add_sem ctx r
+    (IN: my_tid < List.length ctx):
+    ctx_sem (ctx_add ctx r) = ctx_sem ctx ⋅ r.
+  Proof.
+    unfold ctx_add, ctx_set. revert my_tid r IN.
+    induction ctx; i; ss; try nia.
+    destruct my_tid; s; r_solve.
+    eapply IHctx; try nia.
+  Qed.
+
+  Lemma le_mine_in (ctx0 ctx: list Σ)
+    (CTXLE: le_mine eq my_tid ctx0 ctx)
+    (IN: my_tid < List.length ctx0)
+    :
+    my_tid < List.length ctx.
+  Proof.
+    unfold le_mine in *.
+    eapply lookup_lt_is_Some_2 in IN. rdes IN.
+    eapply CTXLE in IN. des. subst.
+    eapply lookup_lt_is_Some_1. eauto.
+  Qed.
+
+  Lemma ctx_set_le_others ctx r:
+    le_others my_tid ctx (ctx_set ctx r).
+  Proof.
+    unfold ctx_set. r; esplits.
+    - rewrite list.insert_length. eauto.
+    - i. rewrite list_lookup_insert_ne; eauto.
+  Qed.
+
+  Lemma ctx_le_mine_sem (w0 w1: list Σ)
+    (IN: my_tid < List.length w0)
+    (LE: le_mine eq my_tid w0 w1)
+    :
+    ctx_sem w1 = ctx_sem (ctx_set w1 (or_else (w0 !! my_tid) ε)).
+  Proof.
+    unfold ctx_sem, ctx_set.
+    move w1 before Ist. revert_until w1.
+    induction w1; i; eauto.
+    destruct w0; ss; try nia.
+    destruct my_tid; ss.
+    - exploit LE; ss. i; des. inv x0. eauto.
+    - erewrite IHw1; eauto. nia.
+  Qed.
+
   Variant interp_inv: list Σ -> nat * Any.t * Any.t -> Prop :=
   | interp_inv_intro
       (ctx: list Σ) (mr_src mr_tgt: Σ) nths st_src st_tgt mr
+      (* (LEN: List.length ctx = nths) *)
       (WF: URA.wf mr_src)
-      (MRS: Own mr_src ⊢ #=> Own ((foldl URA.add ε ctx) ⋅ mr ⋅ mr_tgt))
+      (MRS: Own mr_src ⊢ #=> Own (ctx_sem ctx ⋅ mr ⋅ mr_tgt))
       (MR: Own mr ⊢ #=> Ist nths st_src st_tgt)
       (NODUPS: List.NoDup (List.map fst st_src))
       (NODUPT: List.NoDup (List.map fst st_tgt))
     :
     interp_inv ctx (nths, Any.pair (alist_encode st_src) mr_src↑, Any.pair (alist_encode st_tgt) mr_tgt↑)
   .
-
+  
   Lemma hpsim_adequacy:
     forall
       (NODUPFS: List.NoDup (List.map fst fl_src))
@@ -703,205 +807,317 @@ Section HPSIM_ADEQUACY.
       (NODUPT: List.NoDup (List.map fst st_tgt))
       (ctx0 ctx: list Σ) (mr_src mr_tgt fr_src fr_tgt fmr: Σ)
       (CTXLE: @le_mine Σ eq my_tid ctx0 ctx)
+      (NTHS: my_tid < List.length ctx0)
       (SIM: hpsim_body fl_src fl_tgt Ist my_tid ps pt nths (st_src, itr_src) (st_tgt, itr_tgt) fmr)
       (WF: URA.wf (fr_src ⋅ mr_src))
-      (FMR: Own (fr_src ⋅ mr_src) ⊢ #=> Own ((foldl URA.add ε ctx) ⋅ fmr ⋅ fr_tgt ⋅ mr_tgt)),
+      (FMR: Own (fr_src ⋅ mr_src) ⊢ #=> Own ((ctx_sem ctx) ⋅ fmr ⋅ fr_tgt ⋅ mr_tgt)),
     @sim_itree fl_src0 fl_tgt0 Σ ε interp_inv eq my_tid ctx0 ps pt ctx nths
       (Any.pair (alist_encode st_src) mr_src↑, interp_hp_body itr_src fr_src)
       (Any.pair (alist_encode st_tgt) mr_tgt↑, interp_hp_body itr_tgt fr_tgt).
   Proof.
-  (*   i. apply hpsim_add_dummy in SIM; cycle 1; eauto. *)
-  (*   revert_until FLT. ginit. gcofix CIH. i. *)
-  (*   remember (st_src, itr_src). remember (st_tgt, itr_tgt). *)
-  (*   move SIM before FLT. revert_until SIM. punfold SIM. *)
-  (*   pattern ps, pt, nths, p, p0, fmr. *)
-  (*   eapply _hpsim_tarski, SIM; i. clear SIM fmr. rename fmr0 into fmr. *)
-  (*   exploit IN; i; des. *)
-  (*   { eapply own_wf in FMR; eauto. rewrite (URA.add_comm _ fmr) in FMR. *)
-  (*     repeat eapply URA.wf_mon in FMR. eauto. } *)
-  (*   assert (URA.wf fmr). *)
-  (*   { eapply own_wf, WF. *)
-  (*     eapply own_trans; et. rewrite <- !URA.add_assoc. *)
-  (*     iIntros "[_ [FMR _]]". eauto. } *)
-  (*   assert (URA.wf fmr0). *)
-  (*   { eapply own_wf; eauto. } *)
-    
-  (*   destruct x0; i; des. *)
-  (*   - unfold interp_hp_body, hp_fun_tail, handle_Guarantee, guarantee, mget_res, mput_res. *)
-  (*     steps. force_l. instantiate (1 := (c0, c1, ctx ⋅ fmr0 ⋅ c)). steps. *)
-  (*     force_l. *)
-  (*     { eapply own_trans; et. rewrite <- !URA.add_assoc. *)
-  (*       iIntros "[CTX [FMR TGT]]". iPoseProof (x with "TGT") as "C". *)
-  (*       iMod "C" as "[[C0 C1] C]". iSplitL "C0"; eauto. *)
-  (*       iSplitL "C1"; eauto. iSplitL "CTX"; eauto. iSplitL "FMR"; eauto. *)
-  (*       iApply x1; eauto. *)
-  (*     } *)
-  (*     steps. force_l; et.  *)
-  (*     steps. econs. *)
-  (*     unfold hpsim_tail in RET. *)
-  (*     esplits; et; cycle 1. *)
-  (*     { eapply own_pure; eauto. *)
-  (*       iIntros "H". iPoseProof (RET with "H") as "[_ EQ]". *)
-  (*       iApply Upd_Pure.  eauto. } *)
-  (*     econs; et; cycle 1. *)
-  (*     { iIntros "H". iPoseProof (RET with "H") as "[H _]". et. } *)
-  (*     eapply own_wf, WF. eapply own_trans; et. rewrite <- !URA.add_assoc. *)
-  (*     iIntros "[CTX [FMR TGT]]". iPoseProof (x with "TGT") as "C". *)
-  (*     iMod "C" as "[[C0 C1] C]". iSplitL "CTX"; eauto. iSplitL "FMR"; eauto. *)
-  (*     iApply x1; eauto. *)
-  (*   - unfold interp_hp_body. *)
-  (*     exploit iProp_sepconj_upd; eauto. i; des. *)
-  (*     rename rq into fr, rp into mr. *)
-  (*     steps_safe. unfold handle_Guarantee, guarantee, mget_res, mput_res. *)
-  (*     steps_safe. rename c1 into frt, c into mrt. *)
-  (*     force_l. instantiate (1:= (ε, ε, c0 ⋅ ctx ⋅ fr ⋅ frt ⋅ mr ⋅ mrt)). *)
-  (*     assert (UPD: Own (ctx ⋅ fmr ⋅ fr_tgt ⋅ mr_tgt) *)
-  (*                   ⊢ #=> Own (c0 ⋅ ctx ⋅ fr ⋅ frt ⋅ mr ⋅ mrt)). *)
-  (*     { rewrite <-!URA.add_assoc. *)
-  (*       iIntros "[CTX [FMR TGT]]". *)
-  (*       iPoseProof (x with "TGT") as "TGT". iMod "TGT". *)
-  (*       iPoseProof (x1 with "FMR") as "FMR". iMod "FMR". *)
-  (*       iPoseProof (x0 with "FMR") as "FMR". iMod "FMR". *)
-  (*       iCombine "CTX FMR TGT" as "RES". iModIntro. iStopProof. *)
-  (*       eapply eq_ind; eauto. f_equal. r_solve. *)
-  (*     } *)
-  (*     steps_safe. force_l. *)
-  (*     { etrans; eauto. r_solve. iIntros "H". iMod "H". iApply UPD. eauto. } *)
-  (*     steps_safe. force_l; et. *)
-  (*     steps_safe. eapply safe_sim_sim; econs. esplits; i. *)
-  (*     { instantiate (1:= ctx ⋅ fr ⋅ frt). econs; cycle 2; eauto. *)
-  (*       { iIntros "H". iApply x2. eauto. } *)
-  (*       { eapply own_wf, WF. etrans. apply FMR. *)
-  (*         iIntros "H". iMod "H". iApply UPD. eauto. } *)
-  (*       { rewrite -!URA.add_assoc URA.add_comm. *)
-  (*         iIntros "H". iModIntro. iStopProof. apply Own_extends. *)
-  (*         r; esplits; eauto. } *)
-  (*     } *)
-  (*     steps_safe. *)
-  (*     inv WF0. eapply K with (fmr0 := fr ⋅ mr0); r_solve; et; i. *)
-  (*     { iIntros "[FR MR]". iSplitR "FR"; [iApply MR|iApply x3]; eauto. } *)
-  (*     { eapply eq_ind; eauto. do 2 f_equal. r_solve. } *)
-  (*   - unfold interp_hp_body. steps. eapply K; et. *)
-  (*     eapply own_upd_in_middle; eauto.  *)
-  (*   - exploit K; cycle 3; eauto; inv Heqp; eauto. *)
-  (*     { eapply own_upd_in_middle; eauto. } *)
-  (*     i. steps. rewrite-> interp_hp_body_bind, interp_hp_call. *)
-  (*     unfold handle_Guarantee, mget_res, mput_res, guarantee.  *)
-  (*     steps. force_l. instantiate (1:= (ε, ε, fr_src ⋅ mr_src)). *)
-  (*     steps. force_l. { r_solve; et. } *)
-  (*     steps. force_l; et. steps. *)
-  (*     {	instantiate (1:= interp_hp_fun f). *)
-  (*     rewrite alist_find_map. rewrite FUN. et. } *)
-  (*     guclo sim_strictC_spec. econs; eauto. *)
-  (*     + unfold interp_hp_fun. grind. *)
-  (*       pattern (` r0 : Any.t <- f varg;; ` x : Any.t <- (trigger (Guarantee True);;; Ret r0);; k_src x). *)
-  (*       replace (` r0 : Any.t <- f varg;; ` x : Any.t <- (trigger (Guarantee True);;; Ret r0);; k_src x) *)
-  (*          with (` x: Any.t <- f varg;; trigger (Guarantee True);;; k_src x); grind. *)
-  (*       apply interp_strict_inline_src. *)
-  (*     + apply sim_strict_refl. *)
-  (*   - exploit K; cycle 3; eauto; inv Heqp0; eauto. *)
-  (*     { eapply own_upd_in_middle; eauto. } *)
-  (*     i. steps. rewrite-> interp_hp_body_bind, interp_hp_call. *)
-  (*     unfold handle_Guarantee, mget_res, mput_res, guarantee.  *)
-  (*     steps.  *)
-  (*     {	instantiate (1:= interp_hp_fun f). *)
-  (*     rewrite alist_find_map. rewrite FUN. et. } *)
-  (*     guclo sim_strictC_spec. econs; eauto. *)
-  (*     + apply sim_strict_refl. *)
-  (*     + unfold interp_hp_fun. grind. *)
-  (*       pattern (` r0 : Any.t <- f varg;; ` x3 : Any.t <- (trigger (Guarantee True);;; Ret r0);; k_tgt x3). *)
-  (*       replace (` r0 : Any.t <- f varg;; ` x3 : Any.t <- (trigger (Guarantee True);;; Ret r0);; k_tgt x3) *)
-  (*          with (` x: Any.t <- f varg;; trigger (Guarantee True);;; k_tgt x); grind. *)
-  (*       apply interp_strict_inline_tgt. eapply own_trans; eauto. *)
-  (*       iIntros "[[C0 C1] C]". iModIntro. iSplitR "C"; eauto. *)
-  (*   - unfold interp_hp_body. steps. eapply K; et. eapply own_upd_in_middle; eauto. *)
-  (*   - unfold interp_hp_body. steps. eapply K; et. eapply own_upd_in_middle; eauto. *)
-  (*   - unfold interp_hp_body. steps. eapply K; et. eapply own_upd_in_middle; eauto. *)
-  (*   - unfold interp_hp_body. steps. eapply K; et. eapply own_upd_in_middle; eauto. *)
-  (*   - unfold interp_hp_body. steps. force_l. steps. eapply K; et. eapply own_upd_in_middle; eauto. *)
-  (*   - unfold interp_hp_body. steps. force_r. steps. eapply K; et. eapply own_upd_in_middle; eauto. *)
-  (*   - unfold interp_hp_body. steps. unfold mput_kv. steps. *)
-  (*     rewrite alist_encode_decode. *)
-  (*     des_ifs. eapply K; eauto. *)
-  (*     + eapply alist_upd_nodup. eauto. *)
-  (*     + eapply own_upd_in_middle; eauto. *)
-  (*   - unfold interp_hp_body. steps. unfold mput_kv. steps. *)
-  (*     rewrite alist_encode_decode. *)
-  (*     des_ifs. eapply K; eauto. *)
-  (*     + eapply alist_upd_nodup. eauto. *)
-  (*     + eapply own_upd_in_middle; eauto. *)
-  (*   - unfold interp_hp_body. steps. unfold mget_kv. steps. *)
-  (*     rewrite alist_encode_decode. *)
-  (*     des_ifs. eapply K; eauto. eapply own_upd_in_middle; eauto. *)
-  (*   - unfold interp_hp_body. steps. unfold mget_kv. steps. *)
-  (*     rewrite alist_encode_decode. *)
-  (*     des_ifs. eapply K; eauto. eapply own_upd_in_middle; eauto. *)
-  (*   - unfold interp_hp_body. steps. rewrite interp_hp_Assume. unfold handle_Assume, mget_res, mput_res. *)
-  (*     steps. eapply K with (fmr0 := x ⋅ fmr0); et. *)
-  (*     { *)
-  (*       iIntros "[X FMR]". iPoseProof (_ASSUME0 with "X") as "iP".  *)
-  (*       iPoseProof (CUR with "FMR") as "FMR". iMod "FMR".  *)
-  (*       iModIntro. iFrame. *)
-  (*     }   *)
-  (*     eapply own_ctx with (ctx := x) in FMR; et. rewrite URA.add_assoc in FMR. *)
-  (*     replace (x ⋅ (ctx ⋅ fmr ⋅ fr_tgt ⋅ mr_tgt)) with (ctx ⋅ x ⋅ fmr ⋅ fr_tgt ⋅ mr_tgt) in FMR; r_solve. *)
-  (*     eapply own_upd_in_middle; eauto. *)
-  (*   - unfold interp_hp_body. steps. *)
-  (*     rewrite interp_hp_Guarantee. unfold handle_Guarantee, guarantee, mget_res, mput_res. *)
-  (*     steps. eapply K with (fmr0 := c0 ⋅ fmr0); et. *)
-  (*     { iIntros "[P FMR]". iPoseProof (x0 with "P") as "P". iPoseProof (CUR with "FMR") as "FMR". iFrame. eauto. } *)
-  (*     eapply own_trans; et. *)
-  (*     replace (ctx ⋅ (c0 ⋅ fmr0) ⋅ c1 ⋅ c) with (ctx ⋅ fmr0 ⋅ (c0 ⋅ c1 ⋅ c)); [|r_solve]. *)
-  (*     rewrite <- URA.add_assoc. eapply own_trans with (b:= (ctx ⋅ fmr ⋅ (c0 ⋅ c1 ⋅ c))). *)
-  (*     { eapply own_ctx. et. } *)
-  (*     iIntros "[[CTX FMR] C]". iPoseProof (x1 with "FMR") as "FMR". iMod "FMR".  *)
-  (*     iModIntro. iSplitR "C"; eauto. iSplitR "FMR"; eauto.  *)
-  (*   - unfold interp_hp_body. steps. *)
-  (*     rewrite interp_hp_Guarantee. assert (H1 := CUR). *)
-  (*     eapply iProp_sepconj_upd in H1; eauto. des. rename rq into fmr1. *)
-  (*     unfold handle_Guarantee, guarantee, mget_res, mput_res. *)
-  (*     steps. force_l. instantiate (1:= (rp, fmr1 ⋅ fr_tgt, ctx ⋅ mr_tgt)). *)
-  (*     steps. force_l.  *)
-  (*     { *)
-  (*       replace (rp ⋅ (fmr1 ⋅ fr_tgt) ⋅ (ctx ⋅ mr_tgt)) with (ctx ⋅ rp ⋅ fmr1 ⋅ fr_tgt ⋅ mr_tgt); r_solve.  *)
-  (*       iIntros "H". iPoseProof (FMR with "H") as "H". iMod "H". *)
-  (*       iDestruct "H" as "[H H0]". iSplitL "H"; et. *)
-  (*       iDestruct "H" as "[H H0]". iSplitL "H"; et. *)
-  (*       rewrite <- URA.add_assoc.  *)
-  (*       iDestruct "H" as "[H H0]". iSplitL "H"; et. *)
-  (*       iStopProof. eapply own_trans; eauto.  *)
-  (*     } *)
-  (*     steps. force_l; eauto using iProp_Own. *)
-  (*     steps. eapply K with (fmr0 := fmr1); et. *)
-  (*     { iIntros "H". iApply H3; eauto. } *)
-  (*     { *)
-  (*       eapply own_wf in FMR; et. *)
-  (*       replace (ctx ⋅ fmr ⋅ fr_tgt ⋅ mr_tgt) with (fmr ⋅ (ctx ⋅ fr_tgt ⋅ mr_tgt)) in FMR; r_solve. *)
-  (*       eapply own_ctx_r in x1, H1. eapply own_wf in x1, H1; eauto. *)
-  (*       replace (rp ⋅ fmr1 ⋅ (ctx ⋅ fr_tgt ⋅ mr_tgt)) with (fmr1 ⋅ fr_tgt ⋅ ctx ⋅ mr_tgt ⋅ rp) in H1; r_solve. *)
-  (*       eapply URA.wf_mon; eauto. *)
-  (*     } *)
-  (*     replace (fmr1 ⋅ fr_tgt ⋅ (ctx ⋅ mr_tgt)) with (ctx ⋅ fmr1 ⋅ fr_tgt ⋅ mr_tgt); r_solve; eauto. *)
-  (*   - unfold interp_hp_body. steps. rewrite interp_hp_Assume. assert (H1 := CUR).  *)
-  (*     eapply iProp_sepconj_upd in H1; eauto. des. rename rq into fmr1. *)
-  (*     unfold handle_Assume, assume, mget_res, mput_res.  *)
-  (*     steps. force_r. instantiate (1:= rp). *)
-  (*     steps. force_r. *)
-  (*     { *)
-  (*       eapply own_wf in FMR; et. replace (ctx ⋅ fmr ⋅ fr_tgt ⋅ mr_tgt) with ((fmr ⋅ (fr_tgt ⋅ mr_tgt) ⋅ ctx)) in FMR; r_solve. *)
-  (*       eapply URA.wf_mon in FMR. eapply own_ctx_r in x1, H1. eapply own_wf in x1, H1; eauto.  *)
-  (*       replace (rp ⋅ fmr1 ⋅ (fr_tgt ⋅ mr_tgt)) with (rp ⋅ fr_tgt ⋅ mr_tgt ⋅ fmr1) in H1; r_solve. *)
-  (*       eapply URA.wf_mon; eauto. *)
-  (*     } *)
-  (*     steps. force_r; eauto using iProp_Own. *)
-  (*     steps. eapply K with (fmr0 := fmr1); eauto using iProp_Own. *)
-  (*     { iIntros "H". iApply H3; eauto. } *)
-  (*     eapply own_trans; eauto. *)
-  (*     eapply own_trans. { eapply own_upd_in_middle; eauto. } *)
-  (*     replace (ctx ⋅ fmr1 ⋅ (rp ⋅ fr_tgt) ⋅ mr_tgt) with (ctx ⋅ (rp ⋅ fmr1) ⋅ fr_tgt ⋅ mr_tgt); [|r_solve]. *)
-  (*     eapply own_upd_in_middle; eauto. *)
-  (*   - steps. pclearbot. gstep. econs. gfinal. left. eapply CIH; et. eapply own_upd_in_middle; eauto. *)
-  (* Qed. *)
-  Admitted.
+    i. apply hpsim_add_dummy in SIM; cycle 1; eauto.
+    revert_until FLT. ginit. gcofix CIH. i.
+    remember (st_src, itr_src). remember (st_tgt, itr_tgt).
+    move SIM before FLT. revert_until SIM. punfold SIM.
+    pattern ps, pt, nths, p, p0, fmr.
+    eapply _hpsim_tarski, SIM; i. clear SIM fmr. rename fmr0 into fmr.
+    exploit IN; i; des.
+    { eapply own_wf in FMR; eauto. rewrite (URA.add_comm _ fmr) in FMR.
+      repeat eapply URA.wf_mon in FMR. eauto. }
+    assert (URA.wf fmr).
+    { eapply own_wf, WF.
+      eapply own_trans; et. rewrite <- !URA.add_assoc.
+      iIntros "[_ [FMR _]]". eauto. }
+    assert (URA.wf fmr0).
+    { eapply own_wf; eauto. }
+
+    destruct x0; i; des.
+    - unfold interp_hp_body, hp_fun_tail, handle_Guarantee, guarantee, mget_res, mput_res.
+      clarify. hide Choose 1. steps. unhide.
+      force_l. instantiate (1 := (c0, c1, (ctx_sem ctx) ⋅ fmr0 ⋅ c)).
+      hide Choose 1. step. unhide.
+      force_l.
+      { eapply own_trans; et. rewrite <- !URA.add_assoc.
+        iIntros "[CTX [FMR TGT]]". iPoseProof (x with "TGT") as "C".
+        iMod "C" as "[[C0 C1] C]". iSplitL "C0"; eauto.
+        iSplitL "C1"; eauto. iSplitL "CTX"; eauto. iSplitL "FMR"; eauto.
+        iApply x1; eauto.
+      }
+      steps. econs; eauto.
+      unfold hpsim_tail in RET.
+      esplits; et; cycle 1.
+      { eapply own_pure; eauto.
+        iIntros "H". iPoseProof (RET with "H") as "[_ EQ]".
+        iApply Upd_Pure.  eauto. }
+      econs; et; cycle 1.
+      { iIntros "H". iPoseProof (RET with "H") as "[H _]". et. }
+      eapply own_wf, WF. eapply own_trans; et. rewrite <- !URA.add_assoc.
+      iIntros "[CTX [FMR TGT]]". iPoseProof (x with "TGT") as "C".
+      iMod "C" as "[[C0 C1] C]". iSplitL "CTX"; eauto. iSplitL "FMR"; eauto.
+      iApply x1; eauto.
+    - unfold interp_hp_body.
+      exploit iProp_sepconj_upd; eauto. i; des.
+      rename rq into fr, rp into mr.
+      steps. unfold handle_Guarantee, guarantee, mget_res, mput_res.
+      hide Choose 1. hide Call 2. steps. unhide.
+      rename c1 into frt, c into mrt.
+      force_l. instantiate (1:= (ε, ε, c0 ⋅ (ctx_sem ctx) ⋅ fr ⋅ frt ⋅ mr ⋅ mrt)).
+      assert (UPD: Own ((ctx_sem ctx) ⋅ fmr ⋅ fr_tgt ⋅ mr_tgt)
+                    ⊢ #=> Own (c0 ⋅ (ctx_sem ctx) ⋅ fr ⋅ frt ⋅ mr ⋅ mrt)).
+      { rewrite <-!URA.add_assoc.
+        iIntros "[CTX [FMR TGT]]".
+        iPoseProof (x with "TGT") as "TGT". iMod "TGT".
+        iPoseProof (x1 with "FMR") as "FMR". iMod "FMR".
+        iPoseProof (x0 with "FMR") as "FMR". iMod "FMR".
+        iCombine "CTX FMR TGT" as "RES". iModIntro. iStopProof.
+        eapply eq_ind; eauto. f_equal. r_solve.
+      }
+      hide Choose 1. hide Call 2. step. unhide.
+      force_l.
+      { etrans; eauto. r_solve. iIntros "H". iMod "H". iApply UPD. eauto. }
+      force_l; et.
+      hide Call 1. hide Call 1. do 2 step. unhide.
+      _step; swap 1 2.
+      { instantiate (1:= (ctx_add ctx (fr ⋅ frt))).
+        econs; cycle 2; eauto.
+        { iIntros "H". iApply x2. eauto. }
+        { eapply own_wf, WF. etrans. apply FMR.
+          iIntros "H". iMod "H". iApply UPD. eauto. }
+        { iIntros "H". iModIntro. iStopProof. apply Own_extends.
+          do 2 apply URA.extends_add.
+          rewrite/__ -!URA.add_assoc [c0 ⋅ _]URA.add_comm.
+          r; esplits. rewrite ctx_add_sem; eauto using le_mine_in.
+        }
+      }
+      { apply ctx_set_le_others. }
+
+      guclo lflagC_spec. econs; try instantiate (1:=ctx_set w1 (or_else (ctx !! my_tid) ε)); eauto; cycle 1.
+      { apply ctx_set_le_others. }
+
+      assert (LT0: my_tid < strings.length ctx).
+      { eauto using le_mine_in. }
+      assert (LT: my_tid < strings.length w1).
+      {
+        eapply le_mine_in; eauto.
+        unfold ctx_add, ctx_set.
+        rewrite list.insert_length. eauto.
+      }
+                              
+      do 2 step. grind.
+      inv WF0. eapply K with (fmr0 := fr ⋅ mr0); r_solve; et; i.
+      { iIntros "[FR MR]". iSplitR "FR"; [iApply MR|iApply x3]; eauto. }
+      { eapply le_mine_trans; [ii; subst; eauto|..]; eauto.
+        ii. esplits; eauto. unfold ctx_set. rewrite IN0. s.
+        rewrite list_lookup_insert; eauto.
+      }
+      { iIntros "H". iMod (MRS with "H") as "H". iModIntro.
+        iStopProof. apply Own_extends.
+        apply URA.extends_add.
+        rewrite/__ -!URA.add_assoc [mr0 ⋅ _]URA.add_comm.
+        erewrite (ctx_le_mine_sem _ w1); try apply WLE; eauto.
+        - unfold ctx_add, ctx_set.
+          rewrite list_lookup_insert; eauto.
+          setoid_rewrite (ctx_set_sem w1 _ (fr ⋅ frt)); eauto.
+          exists ε. r_solve.
+        - unfold ctx_add, ctx_set. rewrite list.insert_length. nia.
+      }
+    - unfold interp_hp_body. do 4 step. grind. eapply K; et.
+      eapply own_upd_in_middle; eauto.
+    - exploit K; cycle 3; eauto; inv Heqp; eauto.
+      { eapply own_upd_in_middle; eauto. }
+      i. rewrite-> interp_hp_body_bind, interp_hp_call.
+      unfold handle_Guarantee, mget_res, mput_res, guarantee.
+      force_l. instantiate (1:= (ε, ε, fr_src ⋅ mr_src)).
+      step. force_l. { r_solve; et. }
+      force_l; et. steps.
+      {	instantiate (1:= interp_hp_fun f).
+        rewrite alist_find_map. rewrite FUN. et. }
+      guclo sim_strictC_spec. econs; eauto.
+      + unfold interp_hp_fun. grind.
+        eapply eq_ind; [eapply interp_strict_inline_src|].
+        do 2 f_equal. grind.
+      + apply sim_strict_refl.
+    - exploit K; cycle 3; eauto; inv Heqp0; eauto.
+      { eapply own_upd_in_middle; eauto. }
+      i. steps. rewrite-> interp_hp_body_bind, interp_hp_call.
+      unfold handle_Guarantee, mget_res, mput_res, guarantee.
+      steps.
+      {	instantiate (1:= interp_hp_fun f).
+      rewrite alist_find_map. rewrite FUN. et. }
+      guclo sim_strictC_spec. econs; eauto.
+      + apply sim_strict_refl.
+      + unfold interp_hp_fun. grind.
+        match goal with [|-_ ?x _] => pattern x end.
+        eapply eq_ind; [eapply interp_strict_inline_tgt|].
+        * eapply own_trans; eauto.
+          iIntros "[[C0 C1] C]". iModIntro. iSplitR "C"; eauto.
+        * do 2 f_equal. grind.
+    - unfold interp_hp_body. steps. eapply K; et. eapply own_upd_in_middle; eauto.
+    - unfold interp_hp_body. steps. eapply K; et. eapply own_upd_in_middle; eauto.
+    - unfold interp_hp_body. steps. eapply K; et. eapply own_upd_in_middle; eauto.
+    - unfold interp_hp_body. steps. eapply K; et. eapply own_upd_in_middle; eauto.
+    - unfold interp_hp_body. steps. eapply K; et. eapply own_upd_in_middle; eauto.
+    - unfold interp_hp_body. steps. eapply K; et. eapply own_upd_in_middle; eauto.
+    - unfold interp_hp_body. steps. unfold mput_kv. steps.
+      rewrite alist_encode_decode.
+      des_ifs. eapply K; eauto.
+      + eapply alist_upd_nodup. eauto.
+      + eapply own_upd_in_middle; eauto.
+    - unfold interp_hp_body. steps. unfold mput_kv. steps.
+      rewrite alist_encode_decode.
+      des_ifs. eapply K; eauto.
+      + eapply alist_upd_nodup. eauto.
+      + eapply own_upd_in_middle; eauto.
+    - unfold interp_hp_body. steps. unfold mget_kv. steps.
+      rewrite alist_encode_decode.
+      des_ifs. eapply K; eauto. eapply own_upd_in_middle; eauto.
+    - unfold interp_hp_body. steps. unfold mget_kv. steps.
+      rewrite alist_encode_decode.
+      des_ifs. eapply K; eauto. eapply own_upd_in_middle; eauto.
+    - unfold interp_hp_body. steps. rewrite interp_hp_Assume. unfold handle_Assume, mget_res, mput_res.
+      steps. eapply K with (fmr0 := x ⋅ fmr0); et.
+      {
+        iIntros "[X FMR]". iPoseProof (_ASSUME0 with "X") as "iP".
+        iPoseProof (CUR with "FMR") as "FMR". iMod "FMR".
+        iModIntro. iFrame.
+      }
+      eapply own_ctx with (ctx := x) in FMR; et. rewrite URA.add_assoc in FMR.
+      replace (x ⋅ (ctx_sem ctx ⋅ fmr ⋅ fr_tgt ⋅ mr_tgt)) with (ctx_sem ctx ⋅ x ⋅ fmr ⋅ fr_tgt ⋅ mr_tgt) in FMR; r_solve.
+      eapply own_upd_in_middle; eauto.
+    - unfold interp_hp_body. steps.
+      rewrite interp_hp_Guarantee. unfold handle_Guarantee, guarantee, mget_res, mput_res.
+      steps. eapply K with (fmr0 := c0 ⋅ fmr0); et.
+      { iIntros "[P FMR]". iPoseProof (x0 with "P") as "P". iPoseProof (CUR with "FMR") as "FMR". iFrame. eauto. }
+      eapply own_trans; et.
+      replace (ctx_sem ctx ⋅ (c0 ⋅ fmr0) ⋅ c1 ⋅ c) with (ctx_sem ctx ⋅ fmr0 ⋅ (c0 ⋅ c1 ⋅ c)); [|r_solve].
+      rewrite <- URA.add_assoc. eapply own_trans with (b:= (ctx_sem ctx ⋅ fmr ⋅ (c0 ⋅ c1 ⋅ c))).
+      { eapply own_ctx. et. }
+      iIntros "[[CTX FMR] C]". iPoseProof (x1 with "FMR") as "FMR". iMod "FMR".
+      iModIntro. iSplitR "C"; eauto. iSplitR "FMR"; eauto.
+    - unfold interp_hp_body. steps.
+      rewrite interp_hp_Guarantee. assert (H1 := CUR).
+      eapply iProp_sepconj_upd in H1; eauto. des. rename rq into fmr1.
+      unfold handle_Guarantee, guarantee, mget_res, mput_res. grind.
+      force_l. instantiate (1:= (rp, fmr1 ⋅ fr_tgt, ctx_sem ctx ⋅ mr_tgt)).
+      do 2 step.
+      {
+        replace (rp ⋅ (fmr1 ⋅ fr_tgt) ⋅ (ctx_sem ctx ⋅ mr_tgt)) with (ctx_sem ctx ⋅ rp ⋅ fmr1 ⋅ fr_tgt ⋅ mr_tgt); r_solve.
+        iIntros "H". iPoseProof (FMR with "H") as "H". iMod "H".
+        iDestruct "H" as "[H H0]". iSplitL "H"; et.
+        iDestruct "H" as "[H H0]". iSplitL "H"; et.
+        rewrite <- URA.add_assoc.
+        iDestruct "H" as "[H H0]". iSplitL "H"; et.
+        iStopProof. eapply own_trans; eauto.
+      }
+      steps. eapply K with (fmr0 := fmr1); et.
+      { iIntros "H". iApply H3; eauto. }
+      {
+        eapply own_wf in FMR; et.
+        replace (ctx_sem ctx ⋅ fmr ⋅ fr_tgt ⋅ mr_tgt) with (fmr ⋅ (ctx_sem ctx ⋅ fr_tgt ⋅ mr_tgt)) in FMR; r_solve.
+        eapply own_ctx_r in x1, H1. eapply own_wf in x1, H1; eauto.
+        replace (rp ⋅ fmr1 ⋅ (ctx_sem ctx ⋅ fr_tgt ⋅ mr_tgt)) with (fmr1 ⋅ fr_tgt ⋅ ctx_sem ctx ⋅ mr_tgt ⋅ rp) in H1; r_solve.
+        eapply URA.wf_mon; eauto.
+      }
+      replace (fmr1 ⋅ fr_tgt ⋅ (ctx_sem ctx ⋅ mr_tgt)) with (ctx_sem ctx ⋅ fmr1 ⋅ fr_tgt ⋅ mr_tgt); r_solve; eauto.
+    - unfold interp_hp_body. steps. rewrite interp_hp_Assume. assert (H1 := CUR).
+      eapply iProp_sepconj_upd in H1; eauto. des. rename rq into fmr1.
+      unfold handle_Assume, assume, mget_res, mput_res.
+      step. instantiate (1:= rp).
+      do 2 step.
+      {
+        eapply own_wf in FMR; et. replace (ctx_sem ctx ⋅ fmr ⋅ fr_tgt ⋅ mr_tgt) with ((fmr ⋅ (fr_tgt ⋅ mr_tgt) ⋅ ctx_sem ctx)) in FMR; r_solve.
+        eapply URA.wf_mon in FMR. eapply own_ctx_r in x1, H1. eapply own_wf in x1, H1; eauto.
+        replace (rp ⋅ fmr1 ⋅ (fr_tgt ⋅ mr_tgt)) with (rp ⋅ fr_tgt ⋅ mr_tgt ⋅ fmr1) in H1; r_solve.
+        eapply URA.wf_mon; eauto.
+      }
+      steps. eapply K with (fmr0 := fmr1); eauto using iProp_Own.
+      { iIntros "H". iApply H3; eauto. }
+      eapply own_trans; eauto.
+      eapply own_trans. { eapply own_upd_in_middle; eauto. }
+      replace (ctx_sem ctx ⋅ fmr1 ⋅ (rp ⋅ fr_tgt) ⋅ mr_tgt) with (ctx_sem ctx ⋅ (rp ⋅ fmr1) ⋅ fr_tgt ⋅ mr_tgt); [|r_solve].
+      eapply own_upd_in_middle; eauto.
+    - unfold interp_hp_body. steps. rewrite !interp_hp_spawn. do 3 step. grind.
+      eapply K; et.
+      + eapply le_mine_trans; [ii; subst; eauto|..]; eauto.
+        ii. esplits; eauto. rewrite lookup_app_l; eauto using le_mine_in.
+      + iIntros "H". iMod (FMR with "H") as "H".
+        unfold ctx_sem. rewrite foldr_app. s. r_solve.
+        iDestruct "H" as "(((CTX & FMR) & FR) & MR)".
+        iMod (x1 with "FMR") as "FMR".
+        iCombine "CTX FR MR FMR" as "H". iModIntro. iStopProof. apply Own_extends.
+        exists ε. r_solve.
+    - unfold interp_hp_body.
+      exploit iProp_sepconj_upd; eauto. i; des.
+      rename rq into fr, rp into mr.
+      steps. unfold handle_Guarantee, guarantee, mget_res, mput_res.
+      hide Choose 1. hide Yield 2. steps. unhide.
+      rename c1 into frt, c into mrt.
+      force_l. instantiate (1:= (ε, ε, c0 ⋅ (ctx_sem ctx) ⋅ fr ⋅ frt ⋅ mr ⋅ mrt)).
+      assert (UPD: Own ((ctx_sem ctx) ⋅ fmr ⋅ fr_tgt ⋅ mr_tgt)
+                    ⊢ #=> Own (c0 ⋅ (ctx_sem ctx) ⋅ fr ⋅ frt ⋅ mr ⋅ mrt)).
+      { rewrite <-!URA.add_assoc.
+        iIntros "[CTX [FMR TGT]]".
+        iPoseProof (x with "TGT") as "TGT". iMod "TGT".
+        iPoseProof (x1 with "FMR") as "FMR". iMod "FMR".
+        iPoseProof (x0 with "FMR") as "FMR". iMod "FMR".
+        iCombine "CTX FMR TGT" as "RES". iModIntro. iStopProof.
+        eapply eq_ind; eauto. f_equal. r_solve.
+      }
+      hide Choose 1. hide Yield 2. step. unhide.
+      force_l.
+      { etrans; eauto. r_solve. iIntros "H". iMod "H". iApply UPD. eauto. }
+      force_l; et.
+      hide Yield 1. hide Yield 1. do 2 step. unhide.
+      _step; swap 1 2.
+      { instantiate (1:= (ctx_add ctx (fr ⋅ frt))).
+        econs; cycle 2; eauto.
+        { iIntros "H". iApply x2. eauto. }
+        { eapply own_wf, WF. etrans. apply FMR.
+          iIntros "H". iMod "H". iApply UPD. eauto. }
+        { iIntros "H". iModIntro. iStopProof. apply Own_extends.
+          do 2 apply URA.extends_add.
+          rewrite/__ -!URA.add_assoc [c0 ⋅ _]URA.add_comm.
+          r; esplits. rewrite ctx_add_sem; eauto using le_mine_in.
+        }
+      }
+      { apply ctx_set_le_others. }
+
+      guclo lflagC_spec. econs; try instantiate (1:=ctx_set w1 (or_else (ctx !! my_tid) ε)); eauto; cycle 1.
+      { apply ctx_set_le_others. }
+
+      assert (LT0: my_tid < strings.length ctx).
+      { eauto using le_mine_in. }
+      assert (LT: my_tid < strings.length w1).
+      {
+        eapply le_mine_in; eauto.
+        unfold ctx_add, ctx_set.
+        rewrite list.insert_length. eauto.
+      }
+                              
+      do 2 step. grind.
+      inv WF0. eapply K with (fmr0 := fr ⋅ mr0); r_solve; et; i.
+      { iIntros "[FR MR]". iSplitR "FR"; [iApply MR|iApply x3]; eauto. }
+      { eapply le_mine_trans; [ii; subst; eauto|..]; eauto.
+        ii. esplits; eauto. unfold ctx_set. rewrite IN0. s.
+        rewrite list_lookup_insert; eauto.
+      }
+      { iIntros "H". iMod (MRS with "H") as "H". iModIntro.
+        iStopProof. apply Own_extends.
+        apply URA.extends_add.
+        rewrite/__ -!URA.add_assoc [mr0 ⋅ _]URA.add_comm.
+        erewrite (ctx_le_mine_sem _ w1); try apply WLE; eauto.
+        - unfold ctx_add, ctx_set.
+          rewrite list_lookup_insert; eauto.
+          setoid_rewrite (ctx_set_sem w1 _ (fr ⋅ frt)); eauto.
+          exists ε. r_solve.
+        - unfold ctx_add, ctx_set. rewrite list.insert_length. nia.
+      }
+    - unfold interp_hp_body. steps. rewrite !interp_hp_tid. do 3 step.
+      eapply K; et. eapply own_upd_in_middle; eauto.
+    - unfold interp_hp_body. steps. rewrite !interp_hp_tid. do 3 step.
+      eapply K; et. eapply own_upd_in_middle; eauto.
+    - subst. pclearbot. gstep. econs. econs; [apply le_others_refl|].
+      gfinal. left. eapply CIH; et. eapply own_upd_in_middle; eauto.
+  Qed.
 
 End HPSIM_ADEQUACY.
